src/SDK/Keyring/AESKeyring.dfy
@@ -18,70 +18,70 @@ module AESKeyringDef {
   import AESEncryption
   import Mat = Materials
 
+  const AUTH_TAG_LEN_LEN := 4;
+  const IV_LEN_LEN       := 4;
+
   class AESKeyring extends KeyringDefs.Keyring {
     const keyNamespace: string
     const keyName: string
     const wrappingKey: seq<uint8>
-    const aesType: Cipher.CipherParams
+    const wrappingAlgorithm: Cipher.CipherParams
 
     predicate Valid() reads this {
         Repr == {this} &&
-        (|wrappingKey| == Cipher.KeyLengthOfCipher(aesType)) &&
-        (aesType in {Cipher.AES_GCM_128, Cipher.AES_GCM_192, Cipher.AES_GCM_256}) &&
+        (|wrappingKey| == Cipher.KeyLengthOfCipher(wrappingAlgorithm)) &&
+        (wrappingAlgorithm in {Cipher.AES_GCM_128, Cipher.AES_GCM_192, Cipher.AES_GCM_256}) &&
         ValidUTF8(keyNamespace) && ValidUTF8(keyName)
     }
 
-    constructor(namespace: string, name: string, key: seq<uint8>, params: Cipher.CipherParams)
-    //TODO Verify that CipherParams contains valid values.
+    constructor(namespace: string, name: string, key: seq<uint8>, wrappingAlg: Cipher.CipherParams)
     requires ValidUTF8(namespace) && ValidUTF8(name)
-    requires params in {Cipher.AES_GCM_128, Cipher.AES_GCM_192, Cipher.AES_GCM_256}
-    requires |key| == Cipher.KeyLengthOfCipher(params)
+    requires wrappingAlg in {Cipher.AES_GCM_128, Cipher.AES_GCM_192, Cipher.AES_GCM_256}
+    requires |key| == Cipher.KeyLengthOfCipher(wrappingAlg)
     ensures keyNamespace == namespace
     ensures keyName == name
     ensures wrappingKey == key
-    ensures aesType == params
+    ensures wrappingAlgorithm == wrappingAlg
     ensures Valid()
     {
       keyNamespace := namespace;
       keyName := name;
       wrappingKey := key;
-      aesType := params;
+      wrappingAlgorithm := wrappingAlg;
       Repr := {this};
     }
 
-    function method AESProviderInfo(iv: seq<uint8>): seq<uint8>
+    function method SerializeProviderInto(iv: seq<uint8>): seq<uint8>
       requires Valid()
-      requires |iv| == aesType.ivLen as int
+      requires |iv| == wrappingAlgorithm.ivLen as int
       reads this
     {
       StringToByteSeq(keyName) +
-        [0, 0, 0, aesType.tagLen * 8] + // tag length in bits
-        [0, 0, 0, aesType.ivLen] + // IV length in bytes
+        [0, 0, 0, wrappingAlgorithm.tagLen * 8] + // tag length in bits
+        [0, 0, 0, wrappingAlgorithm.ivLen] + // IV length in bytes
         iv
     }
 
     method OnEncrypt(encMat: Mat.EncryptionMaterials) returns (res: Result<Mat.EncryptionMaterials>)
       requires encMat.Valid()
-      requires Valid() ensures Valid()
+      requires Valid()
       modifies encMat`plaintextDataKey
       modifies encMat`encryptedDataKeys
+      ensures Valid()
       ensures res.Success? ==> res.value.Valid() && res.value == encMat
       ensures res.Success? && old(encMat.plaintextDataKey.Some?) ==> res.value.plaintextDataKey == old(encMat.plaintextDataKey)
       ensures res.Failure? ==> unchanged(encMat)
     {
       var dataKey := encMat.plaintextDataKey;
-      var algSuiteID := encMat.algorithmSuiteID;
       if dataKey.None? {
-        var k := Cipher.RNG.GenBytes(AlgorithmSuite.InputKeyLength(algSuiteID) as uint16);
+        var k := Cipher.RNG.GenBytes(encMat.algorithmSuiteID.KeyLength() as uint16);
         dataKey := Some(k);
       }
-      var iv := Cipher.RNG.GenBytes(aesType.ivLen as uint16);
-      var aad := if encMat.encryptionContext.Some?
-                 then Mat.FlattenSortEncCtx(encMat.encryptionContext.get)
-                 else []; //FIXME this is a hack, and I hate it.
-      var encryptResult := AESEncryption.AES.aes_encrypt(aesType, iv, wrappingKey, dataKey.get, aad);
+      var iv := Cipher.RNG.GenBytes(wrappingAlgorithm.ivLen as uint16);
+      var aad := Mat.FlattenSortEncCtx(encMat.encryptionContext);
+      var encryptResult := AESEncryption.AES.aes_encrypt(wrappingAlgorithm, iv, wrappingKey, dataKey.get, aad);
       if encryptResult.Failure? { return Failure("Error on encrypt!"); }
-      var providerInfo := AESProviderInfo(iv);
+      var providerInfo := SerializeProviderInto(iv);
       var edk := Mat.EncryptedDataKey(keyNamespace, providerInfo, encryptResult.value);
       encMat.plaintextDataKey := dataKey;
       encMat.encryptedDataKeys := encMat.encryptedDataKeys + [edk];
@@ -90,22 +90,21 @@ module AESKeyringDef {
 
     predicate method ValidProviderInfo(info: seq<uint8>)
     {
-      //TODO Replace 4s with descriptive constants for auth tag length length, and IV length length
-      |info| == |keyName| + 4 + 4 + 12 &&
+      |info| == |keyName| + AUTH_TAG_LEN_LEN + IV_LEN_LEN + wrappingAlgorithm.ivLen as int &&
       ByteSeqToString(info[0..|keyName|]) == keyName &&
-      seqToUInt32(info[|keyName|..|keyName| + 4]) == aesType.tagLen as uint32 &&
-      seqToUInt32(info[|keyName| + 4 .. |keyName| + 4 + 4]) == aesType.ivLen as uint32
+      SeqToUInt32(info[|keyName|..|keyName| + AUTH_TAG_LEN_LEN]) == wrappingAlgorithm.tagLen as uint32 &&
+      SeqToUInt32(info[|keyName| + AUTH_TAG_LEN_LEN .. |keyName| + AUTH_TAG_LEN_LEN + IV_LEN_LEN]) == wrappingAlgorithm.ivLen as uint32
     }
 
     function method GetIvFromProvInfo(info: seq<uint8>): seq<uint8>
       requires ValidProviderInfo(info)
     {
-      info[|keyName| + 8 ..]
+      info[|keyName| + AUTH_TAG_LEN_LEN + IV_LEN_LEN ..]
     }
 
     method OnDecrypt(decMat: Mat.DecryptionMaterials, edks: seq<Mat.EncryptedDataKey>) returns (res: Result<Mat.DecryptionMaterials>)
       requires Valid() 
-      //requires x.Valid() //TODO Uncomment when valid is defined.
+      requires decMat.Valid()
       modifies decMat`plaintextDataKey
       ensures Valid()
       ensures old(decMat.plaintextDataKey.Some?) ==> res.Success? &&
@@ -123,13 +122,11 @@ module AESKeyringDef {
       while i < |edks| {
         if edks[i].providerID == keyNamespace && ValidProviderInfo(edks[i].providerInfo) {
           var iv := GetIvFromProvInfo(edks[i].providerInfo);
-          var flatEncCtx: seq<uint8> := if decMat.encryptionContext.Some?
-                                        then Mat.FlattenSortEncCtx(decMat.encryptionContext.get)
-                                        else []; //FIXME this is a hack, and I hate it.
-          var decryptResult := AESEncryption.AES.aes_decrypt(aesType, Cipher.TAG_LEN, wrappingKey, edks[0].ciphertext, iv, flatEncCtx);
+          var flatEncCtx: seq<uint8> := Mat.FlattenSortEncCtx(decMat.encryptionContext);
+          var decryptResult := AESEncryption.AES.aes_decrypt(wrappingAlgorithm, wrappingKey, edks[0].ciphertext, iv, flatEncCtx);
           if decryptResult.Success? {
             var ptKey := decryptResult.value;
-            if |ptKey| == AlgorithmSuite.InputKeyLength(decMat.algorithmSuiteID) { // check for correct key length
+            if |ptKey| == decMat.algorithmSuiteID.KeyLength() { // check for correct key length
               decMat.plaintextDataKey := Some(ptKey);
               return Success(decMat);
             }
